backends/lean/Aeneas/Tactic/Step/Step.lean
@@ -2188,7 +2188,7 @@ h1 : ∀ (i : ℕ) (x : i < s.length), s'[i] = 0#u32
         intros y
         apply Lean.Order.admissible_apply (fun _ fx => WP.dspec fx _)
         apply Lean.Order.admissible_flatOrder
-        simp only [WP.dspec]
+        simp only [WP.dspec, WP.pspec]
       · intros
         simp only
         split
